[2023/2/21 report version] ModularProgramTheory.v added.

Babel/MetaProgram/ModularProgramTheory.v
@@ -1,25 +1,281 @@
 (** ModularProgramTheory.v *)
 From Babel Require Import TerminalDogma 
-                          ExtraDogma.Extensionality.
+                          ExtraDogma.Extensionality
+                          ExtraDogma.AllDecidable
+                          POrderFacility.
 
+From Babel Require Import Ranko
+                            ExtensionalityCharacter
+                            AllDecidableCharacter
+                            ClassicalCharacter.
 
-From Coq Require Import Classical.
+From Coq Require Import Relations Classical.
 
 
 Set Implicit Arguments.
 Unset Strict Implicit.
 Unset Printing Implicit Defensive.
 
+Coercion decide_oracle : Sortclass >-> bool.
+
+Notation "⌈ P ⇒ Q ⌉" := (forall s, P s ⊑ Q s).
+
+
+Lemma fun_impl_trans (X : Type) (Y : poset) (P Q R : X -> Y) : 
+
+    ⌈ P ⇒ Q ⌉ -> ⌈ Q ⇒ R ⌉ -> ⌈ P ⇒ R ⌉.
+
+Proof. ranko. transitivity (Q s); ranko. Qed.
+
+Import FunPointwiseOrder.CanonicalStruct.
+
+Module LangModel.
+
+
+(** Meta-language type 
+    Specifies the language specifications for a backward semantics language 
+    model. *)
+Record metaType : Type := {
+    (** The type of data structure. *)
+    Stt : Type;
+    (** The type of assertions (complete lattice required). *)
+    Asn : clattice;
+    (** The type of satisfaction value (complete lattice required). *)
+    SVal : clattice;
+    (** The function to evaluate the satisfaction value. *)
+    sat_eval : Asn -> Stt -> SVal;
+    (** The consistency between [Asn] order and [SVal] order *)
+    sat_eval_consistent : 
+        forall (P Q : Asn), P ⊑ Q <-> ⌈ sat_eval P ⇒ sat_eval Q ⌉;
+}.
+
+(** program language model (with meta type) *)
+Record feature (mT : metaType) : Type := {
+
+    (* the program syntax type *)
+    syntax : Type;
+
+    (* the denotational semantics of the program *)
+    wp : syntax -> Asn mT -> Asn mT;
+
+    prog_monotonic : forall p: syntax, MonotonicFun.mixin_of (wp p);
+}.
+
+(** wp extensionality in the meta level *)
+Axiom wp_extensionality :
+        forall (mT : metaType) (L : feature mT) (p q : syntax L), 
+            wp p = wp q -> p = q.
+
+
+Lemma prog_porderMixin (mT : metaType) (L : feature mT): 
+    Poset.mixin_of (syntax L).
+Proof.
+    refine (@Poset.Mixin (syntax L) (fun s1 s2 => wp s1 ⊑ wp s2) _).
+    constructor.
+    rewrite /reflexive. ranko. by apply (@poset_refl (Asn mT)).
+    rewrite /transitive. ranko. by apply (poset_trans (H x0) (H0 x0)).
+    rewrite /antisymmetric. ranko.
+        apply wp_extensionality. 
+        apply poset_antisym. ranko. ranko.
+Defined.
+
+Canonical prog_porder (mT : metaType) (L : feature mT) := 
+    Poset (syntax L) (@prog_porderMixin mT L).
+
+End LangModel.
+
+Import LangModel.
+
+
+
+
+
+Module SpecMod.
+
+Record syntax (mT : metaType) : Type := {
+    pre: Asn mT;
+    post: Asn mT;
+}.
+
+Definition wp (mT : metaType) : syntax mT -> Asn mT -> Asn mT :=
+    fun p => fun R => 
+        if post p ⊑ R 
+            then pre p 
+            else ⊔ᶜˡ ∅.
+
+Lemma prog_monotonic (mT : metaType) : 
+    forall p: syntax mT, MonotonicFun.mixin_of (wp p).
+Proof.
+    rewrite /MonotonicFun.mixin_of => p P Q.
+    rewrite /wp => H.
+
+    case E: (decide_oracle (post p ⊑ P)).
+    - rewrite decide_oracle_true in E.
+        replace (decide_oracle (post p ⊑ Q)) with true.
+        by reflexivity.
+        symmetry. rewrite decide_oracle_true. by transitivity P.
+    - apply CLattice.join_prop. ranko.
+Qed.
+
+
+Definition specMod (mT : metaType) : feature mT := {|
+    LangModel.syntax := syntax mT;
+    LangModel.wp := @wp mT;
+    LangModel.prog_monotonic := @prog_monotonic mT;
+|}.
+
+
+Module RefinementFactory.
+(** Language model obtained after equiping it with specification refinement. *)
+(** The program syntax. *)
+Inductive prog_with_spec (mT : metaType) (L : feature mT) : Type :=
+| prog_part (p : LangModel.syntax L)
+| spec_part (s : LangModel.syntax (specMod mT)).
+
+(** The wp semantics. *)
+Definition wp_with_spec (mT : metaType) (L : feature mT) : 
+        prog_with_spec L -> Asn mT -> Asn mT :=
+    fun p => fun R =>
+        match p with
+        | prog_part p' => LangModel.wp p' R
+        | spec_part s => wp s R
+        end.
+
+(** The prog_monotonic proof *)
+Lemma prog_with_spec_monotonic (mT : metaType) (L : feature mT) : 
+        forall p: prog_with_spec L, MonotonicFun.mixin_of (wp_with_spec p).
+Proof.
+    case.
+    ranko.
+    by apply prog_monotonic.
+Qed.
+
+Definition type (mT : metaType) (L : feature mT) : feature mT := {|
+    LangModel.syntax := prog_with_spec L;
+    LangModel.wp := @wp_with_spec _ L;
+    LangModel.prog_monotonic := @prog_with_spec_monotonic _ L;
+|}.
+
+End RefinementFactory.
+
+
+
+
+Module Exports.
+
+Notation "P ‖ Q" := {| pre := P; post := Q |} (at level 50).
+(* #[export] Hint Unfold RefinementFactory.wp_with_spec : magic_book. *)
+
+End Exports.
+
+End SpecMod.
+Import SpecMod.Exports.
+
+
+Check (prog_porder (SpecMod.specMod _)).
+
+
+
+Theorem Theorem_Refinement_A (mT : metaType) 
+        (L : feature mT) (P Q : Asn mT) 
+        (s : syntax (SpecMod.RefinementFactory.type L)): 
+
+        (SpecMod.RefinementFactory.spec_part L (P ‖ Q) 
+            : (prog_porder (SpecMod.RefinementFactory.type L))) ⊑ s 
+            <-> P ⊑ wp s Q.
+Proof. split.
+    * ranko. 
+    rewrite /FunPointwiseOrder.fun_ord in H. move: H. ranko.
+    refine (poset_trans _ (H Q)).
+    rewrite /SpecMod.wp.
+    replace (decide_oracle (SpecMod.post (P ‖ Q) ⊑ Q))
+        with true.
+        + by apply poset_refl.
+        + symmetry. rewrite decide_oracle_true. ranko. 
+            by apply (@poset_refl (Asn mT)).
+    *
+        ranko. rewrite /FunPointwiseOrder.fun_ord. ranko.
+        rewrite /SpecMod.wp.
+        destruct (decide_oracle (SpecMod.post (P ‖ Q) ⊑ x)) eqn: E.
+        + move: H E. ranko.
+            apply (poset_trans H).
+            apply SpecMod.RefinementFactory.prog_with_spec_monotonic.
+            by apply E.
+        + apply (CLattice.join_prop (CLattice.class (Asn mT))).
+            ranko.
+Qed.
+            
+
+Theorem Theorem_Refinement_B (mT : metaType) 
+        (L : feature mT) (P Q : Asn mT) 
+        (s : syntax (SpecMod.RefinementFactory.type L)): 
+
+        P ⊑ wp s Q <-> ⌈ sat_eval P ⇒ sat_eval (wp s Q) ⌉.
+
+Proof. ranko. Qed.
+
+
+Axiom assign_feature : forall (mT : metaType), feature mT.
+Axiom seq_feature : forall (mT : metaType), feature mT -> feature mT.
+
+Definition lang (mT : metaType) := seq_feature (assign_feature mT).
+Definition lang' (mT : metaType) := seq_feature (seq_feature (assign_feature mT)).
+
+Inductive is_lang (mT : metaType) : feature mT -> Prop := 
+| is_assign : is_lang (assign_feature mT) 
+| is_seq (L : feature mT) (H : is_lang L) : is_lang (seq_feature L)
+
+| is_spec : is_lang (SpecMod.specMod mT).
+
+(** Axiom is_lange spec : this is very convenient!*)
+
+
+
+Theorem Theorem_Refinement' (mT : metaType) 
+        (L : feature mT) (s : syntax L) (P Q : Asn mT) : 
+        wp (P ‖ Q : syntax (SpecMod.specMod _)) ⊑ wp (s)
+            <-> P ⊑ wp s Q.
+Proof. split.
+    * ranko. refine (poset_trans _ (H Q)).
+        rewrite /SpecMod.wp.
+        replace (decide_oracle (SpecMod.post (P ‖ Q) ⊑ Q)) with true.
+        by apply poset_refl.
+        ranko. by apply (@poset_refl (Asn mT)).
+    * ranko. rewrite /SpecMod.wp.
+        case E: (decide_oracle (SpecMod.post (P ‖ Q) ⊑ x)); move : E.
+        + ranko. apply (prog_monotonic s) in E.
+        by refine (poset_trans H _).
+        + ranko. apply (@CLattice.join_prop (Asn mT)). ranko.
+Qed. 
+
+
+
+
+
+
+
+
+
+
+
+
+
+
+
+
+
+
+(*
 
 (** program language model (typed) 
     stt : the variable state type considered in this model *)
 Record prog_lan_model (stt : Type) : Type := {
 
     (* the program syntax type *)
-    prog : Type;
+    syntax : Type;
     
     (* the denotational semantics of the program *)
-    desem : prog -> stt -> stt;
+    desem : syntax -> stt -> stt;
 
 }.
 
@@ -36,7 +292,7 @@ Definition pred_order {stt : Type} (P Q : pred stt) : Prop :=
 
 Record correctness_formula {stt : Type} (plm : prog_lan_model stt) := {
     pre_cond : pred stt;
-    mid_prog : prog plm;
+    mid_prog : syntax plm;
     post_cond : pred stt;
 }.
 
@@ -59,12 +315,12 @@ Definition completeness {stt : Type} {plm : prog_lan_model stt}
 
 (** Being a weakest liberal condition *)
 Definition wlp {stt : Type} {plm : prog_lan_model stt} 
-            (P : pred stt) (S0 : prog plm) (Q : pred stt) :=
+            (P : pred stt) (S0 : syntax plm) (Q : pred stt) :=
     semantic_correct {| pre_cond := P; mid_prog := S0; post_cond := Q |}
     /\ forall P', semantic_correct {| pre_cond := P; mid_prog := S0; post_cond := Q |}
         -> pred_order P' P.
     
-
+*)
 
 
 
@@ -73,7 +329,7 @@ Definition wlp {stt : Type} {plm : prog_lan_model stt}
 
 (** About sequential composition *)
 Inductive prog_seq (plm : prog_lan_model) : Type :=
-| seq_atom (S1 : prog plm)
+| seq_atom (S1 : syntax plm)
 | seq_comp (S1 S2 : prog_seq plm).
 
 Fixpoint desem_seq (plm : prog_lan_model) (P : prog_seq plm) : 
@@ -86,7 +342,7 @@ Fixpoint desem_seq (plm : prog_lan_model) (P : prog_seq plm) :
 Definition seq_cpt (plm : prog_lan_model) : prog_lan_model :=
 {|
     stt := stt plm;
-    prog := prog_seq plm;
+    syntax := prog_seq plm;
     desem := @desem_seq plm;
 |}.
 
